Proved semantic of Head Pattern

theories/Head.v
@@ -21,9 +21,11 @@ Definition heads_aux (G: map_cfg) id b acc : list (blk*map_cfg) :=
 
 Definition heads (G: map_cfg): list (blk*map_cfg) := fold (heads_aux G) G [].
 
-Definition head_sem (G G':map_cfg) (b:blk) :=
-  G' ≡ (remove_id b G) /\ wf_map_cfg G' /\
-  MapsTo_id b G /\ Empty (predecessors b.(blk_id) G).
+Definition head_aux_sem (G0 G G': map_cfg) b :=
+  G' = (remove_id b G0) /\ wf_map_cfg G' /\
+  MapsTo_id b G /\ Empty (predecessors b.(blk_id) G0).
+
+Definition head_sem (G G':map_cfg) (b:blk) := head_aux_sem G G G' b.
 
 (* Lemmas *)
 
@@ -73,8 +75,65 @@ Proof.
   - intro HC. contradict HC. intro HC. eapply empty_mapsto_iff. apply HC.
 Qed.
 
+Lemma head_aux_sem_eq: forall G0 G G' G1 b, G' ≡ G -> head_aux_sem G0 G G1 b <-> head_aux_sem G0 G' G1 b.
+Proof.
+  intros GO G G' G1 b Heq. assert (Heq': G ≡ G') by now symmetry.
+  split; intros [H1 [Hwf1 [Hb Hp]]]; repeat split; trivial;
+  eapply MapsTo_m; try apply Heq; try apply Heq'; try reflexivity; trivial.
+Qed.
+
+Lemma heads_aux_correct:
+  forall G G0 G' b, wf_map_cfg G -> wf_map_cfg G0 ->
+  (b, G') ∈ (fold (heads_aux G0) G []) <-> head_aux_sem G0 G G' b.
+Proof.
+  intros G G0. apply fold_rec_bis.
+  - intros G1 G2 a Heq Hrec G' B Hwf2 Hwf0. setoid_rewrite head_aux_sem_eq. 2:apply Heq.
+    apply Hrec; [apply (wf_map_cfg_eq G2)|];trivial. now symmetry.
+  - intros. split. try contradiction. intros [_ [_ [Hb _]]].
+    now apply empty_mapsto_iff in Hb.
+  - intros idB B a G1 HB HnI Hrec G2 A Hwfa Hwf0.
+    assert (HidB: B.(blk_id) = idB). apply Hwfa. now apply add_1. subst idB.
+    split.
+    * unfold heads_aux. remember (is_empty (predecessors B.(blk_id) G0)) as b. induction b. intros [H|H].
+      + apply pair_equal_spec in H as [H1 H2].
+        subst A G2. repeat split; trivial.
+        -- now apply remove_wf_map_cfg.
+        -- now apply add_1.
+        -- now apply is_empty_iff.
+      + assert (Hh1: (head_aux_sem G0 G1 G2 A)). { 
+          apply Hrec; trivial.
+          eapply wf_map_cfg_eq. 2: {apply remove_wf_map_cfg. apply Hwfa. } symmetry. apply remove_add_elim1; trivial.
+        } destruct Hh1 as [H2 [Hwf2 [HA Hp]]]. repeat split; trivial.
+        case (eq_dec A.(blk_id) B.(blk_id)); unfold eq; intro He.
+        -- contradict HnI. exists A. apply eq_eq in He. now rewrite <- He.
+        -- eapply add_2. now apply neq_sym. trivial.
+      + intro H. assert (Hh1: (head_aux_sem G0 G1 G2 A)). { 
+          apply Hrec; trivial.
+          eapply wf_map_cfg_eq. 2: {apply remove_wf_map_cfg. apply Hwfa. } symmetry. apply remove_add_elim1; trivial.
+        } destruct Hh1 as [H2 [Hwf2 [HA Hp]]]. repeat split; trivial.
+        case (eq_dec A.(blk_id) B.(blk_id)); unfold eq; intro He.
+        -- contradict HnI. exists A. apply eq_eq in He. now rewrite <- He.
+        -- eapply add_2. now apply neq_sym. trivial.
+    * intros [H2 [Hwf2 [HA Hp]]]. unfold heads_aux.
+      remember (is_empty (predecessors B.(blk_id) G0)) as b. induction b.
+      case (eq_dec A.(blk_id) B.(blk_id)); unfold eq; intro H. left.
+      assert (HAB: A=B). {
+        eapply MapsTo_fun. apply HA. apply eq_eq in H. rewrite H. now apply add_1.
+      }
+      + now subst.
+      + right. apply Hrec. eapply wf_map_cfg_add. apply HnI. apply Hwfa. trivial.
+         repeat split; trivial. eapply add_3. apply neq_sym. apply H. apply HA.
+      + apply Hrec. eapply wf_map_cfg_add. apply HnI. apply Hwfa. trivial.
+         repeat split; trivial. case (eq_dec A.(blk_id) B.(blk_id)); unfold eq; intro H.
+         -- assert (HAB: A=B). {
+              eapply MapsTo_fun. apply HA. apply eq_eq in H. rewrite H. now apply add_1.
+            } subst A. apply is_empty_iff in Hp. rewrite Hp in Heqb. discriminate.
+         -- eapply add_3. apply neq_sym. apply H. apply HA.
+Qed.
+
 Lemma heads_correct:
   forall G G' b, wf_map_cfg G ->
   (b, G') ∈ (heads G) <-> head_sem G G' b.
 Proof.
-Admitted.
+  intros. now apply heads_aux_correct.
+Qed.
