theories/MapCFG.v
@@ -38,8 +38,8 @@ Notation single b := (add_id b empty).
 
 Definition wf_map_cfg (g: map_cfg) := forall id b, MapsTo id b g -> b.(blk_id) = id.
 
-
 (* Proofs *)
+
 
 Lemma add_wf_map_cfg: forall b g, wf_map_cfg g -> wf_map_cfg (add_id b g).
 Proof.
@@ -47,6 +47,14 @@ Proof.
   apply add_mapsto_iff in H. destruct H as [[H1 H2]|[H1 H2]].
   - apply eq_eq in H1. now subst.
   - now apply Hwf.
+Qed.
+
+Lemma wf_map_cfg_add: forall id b g, ~In id g -> wf_map_cfg (add id b g) -> wf_map_cfg g.
+Proof.
+  intros idB B G HnI Hwfa idA A HA.
+  apply Hwfa. apply add_2. intro. contradict HnI.
+  exists A. eapply MapsTo_m. apply H.
+  reflexivity. reflexivity. trivial. trivial.
 Qed.
 
 Lemma remove_wf_map_cfg: forall id g, wf_map_cfg g -> wf_map_cfg (remove id g).
@@ -67,6 +75,15 @@ Lemma wf_map_cfg_part:
   wf_map_cfg G -> wf_map_cfg G1 /\ wf_map_cfg G2.
 Proof.
   intros G G1 G2 [Hd Hs] Hwf. split; intros id b Hm; apply Hwf; apply Hs; auto.
+Qed.
+
+Lemma wf_map_cfg_blk:
+  forall G A idA B, wf_map_cfg G -> MapsTo idA A G -> MapsTo A.(blk_id) B G -> A=B.
+Proof.
+  intros.
+  assert (B.(blk_id)=A.(blk_id)) by now apply H.
+  assert (A.(blk_id)=idA) by now apply H. subst.
+  eapply MapsTo_fun. apply H0. trivial.
 Qed.
 
 Lemma add_remove_elim1:
@@ -94,6 +111,17 @@ Proof.
   now symmetry.
 Qed.
 
+Lemma remove_add_elim1:
+  forall id B (G: map_cfg), ~In id G -> G ≡ (remove id (add id B G)).
+Proof.
+  intros idB B G HnI. apply Equal_mapsto_iff. intros idA A.
+  split; intros H; case (eq_dec idA idB); intro H'.
+  - apply eq_eq in H'. subst. contradict HnI. now exists A.
+  - eapply remove_2. now apply neq_sym. apply add_2;trivial. now apply neq_sym.
+  - apply eq_eq in H'. subst. contradict H. intro H. eapply remove_1. reflexivity. exists A. apply H.
+  - eapply add_3. apply neq_sym. apply H'. eapply remove_3. apply H.
+Qed.
+
 Lemma swap_add:
   forall id id' B B' (G : map_cfg), ~ id === id' ->
   (add id B (add id' B' G)) ≡ (add id' B' (add id B G)).
@@ -101,28 +129,29 @@ Proof.
   intros id id' B B' G Hn.
   apply Equal_mapsto_iff. intros k e.
   induction (eq_dec k id) as [b|b]. 2: induction (eq_dec k id') as [b'|b'].
-  - apply eq_eq in b. subst k.
-    split; intro H. assert (He: B=e).
-    apply add_mapsto_iff in H as [[H1 H2]|[H1 H2]]. trivial. contradict H1. apply eq_refl. subst e.
-    apply add_2.
-      * now apply neq_sym. 
-      * apply add_mapsto_iff. left.
-        apply add_mapsto_iff in H as [|[H1 H2]]. trivial. contradict H1. reflexivity.
-      * assert (He: B=e).
+  - apply eq_eq in b. subst.
+    split; intro H.
+    * assert (He: B=e). {
+        apply add_mapsto_iff in H as [[H1 H2]|[H1 H2]]. trivial. contradict H1. apply eq_refl.
+      } subst.
+      apply add_2. now apply neq_sym.
+      apply add_mapsto_iff. left. now split.
+    * assert (He: B=e). {
         apply add_3 in H. apply add_mapsto_iff in H as [[H1 H2]|[H1 H2]].
-        trivial. contradict H1. reflexivity.
-        now apply neq_sym.
-        subst e.
-        apply add_1. reflexivity.
+        trivial. contradict H1. reflexivity. now apply neq_sym.
+      } subst.
+      apply add_1. reflexivity.
   - apply eq_eq in b'. subst.
     split; intro H.
-    * assert (He: B'=e).
-      apply add_3 in H. apply add_mapsto_iff in H as [[H1 H2]|[H1 H2]].
-      trivial. contradict H1. reflexivity. trivial.
-      subst.
+    * assert (He: B'=e). {
+        apply add_3 in H. apply add_mapsto_iff in H as [[H1 H2]|[H1 H2]].
+        trivial. contradict H1. reflexivity. trivial.
+      } subst.
       apply add_1. reflexivity.
-    * assert (He: B'=e). apply add_mapsto_iff in H as [[H1 H2]|[H1 H2]].
-      trivial. contradict H1. reflexivity. subst e.
+    * assert (He: B'=e). {
+        apply add_mapsto_iff in H as [[H1 H2]|[H1 H2]].
+        trivial. contradict H1. reflexivity.
+      } subst e.
       apply add_2. trivial. apply add_1. reflexivity.
   - split; intro H.
     * assert (H': MapsTo k e G).
